\section{Proof Goals}

\begin{leanProofGoal}{126}{56}
⊢ ∀ (n m : nat), add n m = add m n
\end{leanProofGoal} 

\begin{leanProofGoal}{127}{8}
n : nat
⊢ ∀ (m : nat), add n m = add m n
\end{leanProofGoal} 

\begin{leanProofGoal}{127}{21}
case zero
⊢ ∀ (m : nat), add nat.zero m = add m nat.zero

case succ
n† : nat
n_ih† : ∀ (m : nat), add n† m = add m n†
⊢ ∀ (m : nat), add n†.succ m = add m n†.succ
\end{leanProofGoal} 

\begin{leanProofGoal}{128}{6}
⊢ ∀ (m : nat), add nat.zero m = add m nat.zero
\end{leanProofGoal} 

\begin{leanProofGoal}{132}{6}
n : nat
ih : ∀ (m : nat), add n m = add m n
⊢ ∀ (m : nat), add n.succ m = add m n.succ
\end{leanProofGoal} 

\begin{leanProofGoal}{133}{10}
n : nat
ih : ∀ (m : nat), add n m = add m n
m : nat
⊢ add n.succ m = add m n.succ
\end{leanProofGoal} 

\begin{leanProofGoal}{133}{23}
case zero
n : nat
ih : ∀ (m : nat), add n m = add m n
⊢ add n.succ nat.zero = add nat.zero n.succ

case succ
n : nat
ih : ∀ (m : nat), add n m = add m n
n† : nat
n_ih† : add n.succ n† = add n† n.succ
⊢ add n.succ n†.succ = add n†.succ n.succ
\end{leanProofGoal} 

\begin{leanProofGoal}{134}{8}
n : nat
ih : ∀ (m : nat), add n m = add m n
⊢ add n.succ nat.zero = add nat.zero n.succ
\end{leanProofGoal} 

\begin{leanProofGoal}{135}{8}
n : nat
ih : ∀ (m : nat), add n m = add m n
m' : nat
ih' : add n.succ m' = add m' n.succ
⊢ add n.succ m'.succ = add m'.succ n.succ
\end{leanProofGoal} 